Wrap constants in sem monad

ref/6 Items And Attributes/6.1 Items/6.1.7 Constant items/1/lib.rs
@@ -1,5 +1,5 @@
-const BIT1: u32 = 1;
-const BIT2: u32 = 2;
+const BIT1: u32 = 1 << 0;
+const BIT2: u32 = 1 << 1;
 
 const BITS: [u32; 2] = [BIT1, BIT2];
 const STRING: &'static str = "bitstring";
