ref/6 Items And Attributes/6.1 Items/6.1.8 Static items/2/lib.rs
@@ -1,0 +1,1 @@
+static LEVELS: u32 = 0;
