thys/fixedbitset/thy.lean
@@ -22,12 +22,11 @@ eval
 attribute bool.bnot [unfold 1]
 
 attribute sem [reducible]
-attribute BITS [reducible]
 
 structure FixedBitSet' [class] (self : FixedBitSet) : Prop :=
-(length_eq : nat.div_ceil (length self) BITS = list.length (Vec.buf (data self)))
+(length_eq : nat.div_ceil (length self) 32 = list.length (Vec.buf (data self)))
 
-lemma div_rem_BITS (n : usize) : div_rem n BITS = some (n / BITS, n % BITS, 0) := rfl
+lemma div_rem_32 (n : usize) : div_rem n 32 = some (n / 32, n % 32, 0) := rfl
 
 attribute core.u32_as_Copy' [constructor]
 attribute core.marker.Copy'._trans_of_to_Copy [unfold 2]
@@ -35,13 +34,13 @@ attribute core.marker.Copy'._trans_of_to_Copy [unfold 2]
 lemma with_capacity_inv (bits : usize) [is_usize bits] :
   sem.terminates_with FixedBitSet' (with_capacity bits) :=
 obtain v k Hfrom_elem Hv, from
-  sem.terminates_with_eq (from_elem_Copy_eq (0 : nat) (nat.div_ceil bits BITS)),
+  sem.terminates_with_eq (from_elem_Copy_eq (0 : nat) (nat.div_ceil bits 32)),
 begin
   rewrite [↑nat.div_ceil at Hfrom_elem],
-  rewrite [↑with_capacity, div_rem_BITS, ↑bool_to_usize],
-  krewrite [if_congr (bool.of_Prop_eq_tt_iff (0 < bits % BITS)) rfl rfl],
-  have bits / BITS + ite (0 < bits % BITS) 1 0 ≤ usize.max, from
-    have bits / BITS ≤ usize.max - 1, from
+  rewrite [↑with_capacity, ↑BITS, div_rem_32, ↑bool_to_usize],
+  krewrite [if_congr (bool.of_Prop_eq_tt_iff (0 < bits % 32)) rfl rfl],
+  have bits / 32 + ite (0 < bits % 32) 1 0 ≤ usize.max, from
+    have bits / 32 ≤ usize.max - 1, from
       nat.div_le_of_le_mul (le.trans (le_pred_of_lt `is_usize bits`) (calc
         usize.max ≤ usize.max + (usize.max - 1 - 1) : le_add_right
               ... = (usize.max - 1) + (usize.max - 1) : by
@@ -49,9 +48,9 @@ begin
                     nat.le_sub_of_add_le (le.trans dec_trivial usize.max_ge_u16_max)),
                   add.comm, nat.add_sub_assoc usize.max_ge_1]
               ... = (usize.max - 1) * 2    : by rewrite [mul.comm, two_mul]
-              ... ≤ (usize.max - 1) * BITS : nat.mul_le_mul !le.refl dec_trivial
+              ... ≤ (usize.max - 1) * 32 : nat.mul_le_mul !le.refl dec_trivial
     )),
-    calc bits / BITS + ite (0 < bits % BITS) 1 0
+    calc bits / 32 + ite (0 < bits % 32) 1 0
           ≤ usize.max - 1 + 1 : add_le_add this
             (ite_prop (λ h, dec_trivial) (λ h, dec_trivial))
       ... = usize.max : nat.sub_add_cancel usize.max_ge_1,
@@ -65,19 +64,19 @@ variables (s : FixedBitSet) (bit : usize)
 premises [FixedBitSet' s] (Hbit_lt : bit < length s)
 include Hbit_lt
 
-lemma bit_div_BITS_lt_data_length : bit / BITS < list.length (Vec.buf (data s)) :=
-calc bit / BITS < nat.div_ceil (length s) BITS :
+lemma bit_div_32_lt_data_length : bit / 32 < list.length (Vec.buf (data s)) :=
+calc bit / 32 < nat.div_ceil (length s) 32 :
 begin
-  cases decidable_lt 0 (length s % BITS) with Hrem Hnotrem,
-  { exact calc bit / BITS ≤ length s / BITS : nat.div_le_div _ (le_of_lt Hbit_lt)
-                      ... < nat.div_ceil (length s) BITS : begin
+  cases decidable_lt 0 (length s % 32) with Hrem Hnotrem,
+  { exact calc bit / 32 ≤ length s / 32 : nat.div_le_div _ (le_of_lt Hbit_lt)
+                      ... < nat.div_ceil (length s) 32 : begin
       apply nat.lt_add_of_pos_right,
       krewrite [if_pos Hrem],
       apply nat.zero_lt_succ,
     end
   },
-  { have length s % BITS = 0, from nat.eq_zero_of_le_zero (le_of_not_gt Hnotrem),
-    have BITS ∣ length s, from nat.dvd_of_mod_eq_zero this,
+  { have length s % 32 = 0, from nat.eq_zero_of_le_zero (le_of_not_gt Hnotrem),
+    have 32 ∣ length s, from nat.dvd_of_mod_eq_zero this,
     apply nat.div_lt_of_lt_mul,
     rewrite [↑nat.div_ceil],
     krewrite [nat.right_distrib, nat.div_mul_cancel this],
@@ -86,21 +85,21 @@ end
   ... = list.length (Vec.buf (data s)) : FixedBitSet'.length_eq s
 
 lemma contains.spec : sem.terminates_with (λ res,
-    option.any (λ b : u32, res = (b &&[32] 2 ^ (bit % BITS) ≠ᵇ 0))
-      (list.nth (Vec.buf (FixedBitSet.data s)) (bit / BITS))
+    option.any (λ b : u32, res = (b &&[32] 2 ^ (bit % 32) ≠ᵇ 0))
+      (list.nth (Vec.buf (FixedBitSet.data s)) (bit / 32))
   ) (contains s bit) :=
 begin
   intro,
   rewrite [↑contains],
   
-  rewrite [↑div_rem,
-    +if_pos (show BITS ≠ (0 : nat), from !nat.succ_ne_zero)],
+  rewrite [↑div_rem, ↑BITS,
+    +if_pos (show 32 ≠ (0 : nat), from !nat.succ_ne_zero)],
   rewrite [↑«collections.vec.Vec<T> as core.ops.Deref».deref, ↑«[T]».get,
     ↑«[T] as core.slice.SliceExt».get],
-  rewrite [checked.shl_1 (show bit % BITS < u32.bits, from !nat.mod_lt dec_trivial)],
+  rewrite [checked.shl_1 (show bit % 32 < u32.bits, from !nat.mod_lt dec_trivial)],
   rewrite [+incr_incr],
-  note H := bit_div_BITS_lt_data_length s bit Hbit_lt,
-  krewrite [@if_congr _ _ _ _ !nat.decidable_lt _ _ _ _ (@bool.of_Prop_eq_tt_iff (bit / BITS < list.length (Vec.buf (FixedBitSet.data s))) !nat.decidable_lt) rfl rfl],
+  note H := bit_div_32_lt_data_length s bit Hbit_lt,
+  krewrite [@if_congr _ _ _ _ !nat.decidable_lt _ _ _ _ (@bool.of_Prop_eq_tt_iff (bit / 32 < list.length (Vec.buf (FixedBitSet.data s))) !nat.decidable_lt) rfl rfl],
   krewrite [if_pos' H],
   rewrite [↑«[T] as core.slice.SliceExt».get_unchecked],
   cases list.nth_eq_some H with b b_eq,
@@ -119,18 +118,18 @@ lemma insert.spec :
     let s' := ret.2 in
     ∃ (h : FixedBitSet' s'), to_set s' = to_set s ∪ '{bit})
   (insert s bit) :=
-have is_bounded_nat BITS (2^(bit % BITS)), from
+have is_bounded_nat 32 (2^(bit % 32)), from
   strictly_increasing_pow dec_trivial (!mod_lt dec_trivial),
 begin
   intro, rewrite [↑insert],
   have bool.bnot (bit <ᵇ FixedBitSet.length s) = bool.tt ↔ ¬(bit < length s),
   by rewrite [!bool.bnot_of_Prop, bool.of_Prop_eq_tt_iff],
   rewrite [if_congr this rfl rfl, if_neg (not_not_intro `bit < length s`), ▸*],
-  have BITS ≠ (0 : nat), from !nat.succ_ne_zero,
-  rewrite [↑div_rem, +if_pos' this],
+  have 32 ≠ (0 : nat), from !nat.succ_ne_zero,
+  rewrite [↑div_rem, ↑BITS, +if_pos' this],
   rewrite [↑«collections.vec.Vec<T> as core.ops.DerefMut».deref_mut, ↑«[T]».get_unchecked_mut],
-  rewrite [checked.shl_1 (show bit % BITS < u32.bits, from !nat.mod_lt dec_trivial)],
-  note bit_valid := bit_div_BITS_lt_data_length s bit Hbit_lt,
+  rewrite [checked.shl_1 (show bit % 32 < u32.bits, from !nat.mod_lt dec_trivial)],
+  note bit_valid := bit_div_32_lt_data_length s bit Hbit_lt,
   cases list.nth_eq_some bit_valid with b b_eq,
   rewrite [b_eq, ▸*],
   cases list.update_eq_some _ bit_valid with l' l'_eq,
@@ -149,7 +148,7 @@ begin
 
     note H := sem.sem_unwrap (contains.spec s' bit' bit'_lt),
     esimp at H,
-    note Hbit'_valid := bit_div_BITS_lt_data_length s bit' bit'_lt,
+    note Hbit'_valid := bit_div_32_lt_data_length s bit' bit'_lt,
     cases list.nth_eq_some ((list.length_update l'_eq)⁻¹ ▸ Hbit'_valid) with b' b'_eq,
     rewrite [b'_eq at H{2}, ▸* at H, H],
     clear H,
@@ -159,11 +158,11 @@ begin
     rewrite [b''_eq at H{2}, ▸* at H, H],
     clear H,
 
-    note H := list.nth_update (bit' / BITS) l'_eq,
+    note H := list.nth_update (bit' / 32) l'_eq,
     rewrite [b''_eq at H, b'_eq at H],
     clear b'_eq,
 
-    cases (_ : decidable (bit / BITS = bit' / BITS)) with same_blk dif_blk,
+    cases (_ : decidable (bit / 32 = bit' / 32)) with same_blk dif_blk,
     { rewrite [if_pos same_blk at H],
       injection H with H,
       have b'' = b, from
@@ -177,9 +176,9 @@ begin
         apply not_imp_not_of_imp eq_zero_of_pow_eq_zero,
         contradiction
       },
-      { have bit % BITS ≠ bit' % BITS, begin
+      { have bit % 32 ≠ bit' % 32, begin
           revert a, apply not_imp_not_of_imp, intro h,
-          rewrite [eq_div_mul_add_mod bit BITS, eq_div_mul_add_mod bit' BITS, h, same_blk],
+          rewrite [eq_div_mul_add_mod bit 32, eq_div_mul_add_mod bit' 32, h, same_blk],
         end,
         rewrite [iff_false_intro `bit' ≠ bit`, +bool.of_Prop_eq_tt_iff, bitand_bitor_distrib_right,
           !bitand_disj_pow this, bitor_zero],
