ref/6 Items And Attributes/6.1 Items/6.1.8 Static items/pre.md
@@ -1,0 +1,1 @@
+No semantic difference from constants without unsafe code or `*Cell`s.
